src/QUIC.Impl.fsti
@@ -1,7 +1,7 @@
 /// An implementation of QUIC.Spec.fst that is concerned only with functional
 /// correctness (no notion of model for now).
 module QUIC.Impl
-
+include QUIC.Impl.Crypto
 include QUIC.Impl.Header.Base
 
 module QSpec = QUIC.Spec
@@ -31,24 +31,7 @@ open EverCrypt.Error
 // ... up to here!
 
 unfold noextract
-let hash_alg = Spec.Hash.Definitions.hash_alg
-
-unfold noextract
-let aead_alg = Spec.Agile.AEAD.alg
-
-unfold noextract
-let lbytes = QSpec.lbytes
-
-/// This is not a cryptographic index; rather, this is just a regular type
-/// index, where instead of indexing on a single algorithm (like, say, AEAD), we
-/// index on two values.
-///
-/// The record is here to limit the profileration of hide/reveal in the stateful
-/// functions, and to give easier projectors (ADL, JP).
-type index = {
-  hash_alg: QSpec.ha;
-  aead_alg: QSpec.ea
-}
+let lbytes = QUIC.Spec.Base.lbytes
 
 // Reexport this function, which was lost in the bundle
 let header_len = QUIC.Impl.Header.Base.header_len
@@ -59,176 +42,6 @@ let header_len = QUIC.Impl.Header.Base.header_len
 type u2 = n:U8.t{U8.v n < 4}
 type u4 = n:U8.t{U8.v n < 16}
 type u62 = n:UInt64.t{UInt64.v n < pow2 62}
-
-/// Boilerplate
-/// -----------
-
-[@CAbstractStruct]
-val state_s: index -> Type0
-
-let state i = B.pointer (state_s i)
-
-val footprint_s: #i:index -> HS.mem -> state_s i -> GTot B.loc
-let footprint (#i:index) (m: HS.mem) (s: state i) =
-  B.(loc_union (loc_addr_of_buffer s) (footprint_s m (B.deref m s)))
-
-let loc_includes_union_l_footprint_s
-  (m: HS.mem)
-  (l1 l2: B.loc) (#a: index) (s: state_s a)
-: Lemma
-  (requires (
-    B.loc_includes l1 (footprint_s m s) \/ B.loc_includes l2 (footprint_s m s)
-  ))
-  (ensures (B.loc_includes (B.loc_union l1 l2) (footprint_s m s)))
-  [SMTPat (B.loc_includes (B.loc_union l1 l2) (footprint_s m s))]
-= B.loc_includes_union_l l1 l2 (footprint_s m s)
-
-/// Ghost accessors (not needing the invariant)
-/// -------------------------------------------
-///
-/// We need to define those, so that we can state a framing lemma for them.
-/// Attempting a new convention to distinguish ghost accessors from stateful
-/// functions: a ``g_`` prefix.
-
-/// See remark for ``g_initial_packet_number`` below.
-val g_traffic_secret: #i:index -> (s: state_s i) ->
-  GTot (Spec.Hash.Definitions.bytes_hash i.hash_alg)
-
-#push-options "--max_ifuel 1" // inversion on hash_alg
-let hash_is_keysized #i (s: state_s i): Lemma
-  (ensures (QSpec.keysized i.hash_alg (S.length (g_traffic_secret s))))
-  [ SMTPat (g_traffic_secret s) ]
-=
-  assert_norm (512 < pow2 61);
-  assert_norm (512 < pow2 125)
-#pop-options
-
-/// Note that this one does *NOT* take the memory as an argument. (This is
-/// because the initial packet number is erased in the concrete state.) Callers
-/// should be able to derive, from this, that the initial packet number remains
-/// the same, thanks to the precise use of footprint_s in encrypt/decrypt.
-val g_initial_packet_number: #i:index -> (s: state_s i) -> GTot QSpec.nat62
-
-/// Invariant
-/// ---------
-
-val invariant_s: (#i:index) -> HS.mem -> state_s i -> Type0
-let invariant (#i:index) (m: HS.mem) (s: state i) =
-  let r = B.frameOf s in
-  ST.is_eternal_region r /\
-  B.loc_includes (B.loc_region_only true r) (footprint m s) /\
-  B.live m s /\
-  B.(loc_disjoint (loc_addr_of_buffer s) (footprint_s m (B.deref m s))) /\
-  invariant_s m (B.get m s 0)
-
-val invariant_loc_in_footprint
-  (#i: index)
-  (s: state i)
-  (m: HS.mem)
-: Lemma
-  (requires (invariant m s))
-  (ensures (B.loc_in (footprint m s) m))
-  [SMTPat (invariant m s)]
-
-
-/// Ghost accessors needing the invariant
-/// -------------------------------------
-
-val g_last_packet_number: #i:index -> (s: state_s i) -> (h: HS.mem { invariant_s h s }) ->
-  GTot (pn: PN.packet_number_t {
-    Secret.v pn >= g_initial_packet_number s
-  })
-
-let incrementable (#i: index) (s: state i) (h: HS.mem { invariant h s }) =
-  Secret.v (g_last_packet_number (B.deref h s) h) + 1 < pow2 62
-
-/// Preserving all the ghost accessors via a single framing lemma only works
-/// because we don't do stack allocation. See comments in
-/// EverCrypt.Hash.Incremental.
-val frame_invariant: #i:index -> l:B.loc -> s:state i -> h0:HS.mem -> h1:HS.mem -> Lemma
-  (requires (
-    invariant h0 s /\
-    B.loc_disjoint l (footprint h0 s) /\
-    B.modifies l h0 h1))
-  (ensures (
-    invariant h1 s /\
-    footprint h0 s == footprint h1 s /\
-    g_last_packet_number (B.deref h0 s) h0 == g_last_packet_number (B.deref h1 s) h0 /\
-    g_traffic_secret (B.deref h0 s) == g_traffic_secret (B.deref h1 s)
-    ))
-  // Assertion failure: unexpected pattern term
-  (*[ SMTPat (B.modifies l h0 h1); SMTPatOr [
-    [ SMTPat (invariant h1 s) ];
-    [ SMTPat (footprint h1 s) ];
-    [ SMTPat (g_aead_key (B.deref h1 s)) ];
-    [ SMTPat (g_counter (B.deref h1 s)) ]
-  ]]*)
-
-
-
-/// Actual stateful API
-/// -------------------
-
-val aead_alg_of_state (#i: G.erased index) (s: state (G.reveal i)): Stack aead_alg
-  (requires (fun h0 -> invariant #(G.reveal i) h0 s))
-  (ensures (fun h0 a h1 ->
-    a == (G.reveal i).aead_alg /\
-    h0 == h1))
-
-val hash_alg_of_state (#i: G.erased index) (s: state (G.reveal i)): Stack hash_alg
-  (requires (fun h0 -> invariant #(G.reveal i) h0 s))
-  (ensures (fun h0 a h1 ->
-    a == (G.reveal i).hash_alg /\
-    h0 == h1))
-
-val last_packet_number_of_state (#i: G.erased index) (s: state (G.reveal i)): Stack PN.packet_number_t
-  (requires fun h0 -> invariant h0 s)
-  (ensures fun h0 ctr h1 ->
-    ctr == g_last_packet_number (B.deref h0 s) h0 /\
-    h0 == h1)
-
-// JP: we could be defensive and allow callers to pass potentially unsupported
-// algorithms; however, this would require a lot more machinery as we would not
-// even be able to state the index type, since index currently has a refinement
-// that the two algorithms are supported. We would have to separate index into
-// index0 and a well-formedness refinement. Not sure it's worth it. We can
-// always perform redundant tests inside the definition of create to be fully
-// defensive.
-inline_for_extraction noextract
-let create_in_st (i:index) =
-  r:HS.rid ->
-  dst: B.pointer (B.pointer_or_null (state_s i)) ->
-  initial_pn:u62 ->
-  traffic_secret:B.buffer U8.t {
-    B.length traffic_secret = Spec.Hash.Definitions.hash_length i.hash_alg
-  } ->
-  ST error_code
-    (requires fun h0 ->
-      // JP: we could require that ``dst`` point to NULL prior to calling
-      // ``create`` (otherwise, it's a memory leak). Other modules don't enforce
-      // this (see AEAD) so for now, let's make the caller's life easier and not
-      // demand anything.
-      ST.is_eternal_region r /\
-      B.live h0 dst /\ B.live h0 traffic_secret /\
-      B.disjoint dst traffic_secret)
-    (ensures (fun h0 e h1 ->
-      match e with
-      | UnsupportedAlgorithm ->
-          B.(modifies loc_none h0 h1)
-      | Success ->
-          let s = B.deref h1 dst in
-          not (B.g_is_null s) /\
-          invariant h1 s /\
-
-          B.(modifies (loc_buffer dst) h0 h1) /\
-          B.fresh_loc (footprint h1 s) h0 h1 /\
-
-          g_initial_packet_number (B.deref h1 s) == U64.v initial_pn
-      | _ ->
-          False))
-
-// The index is passed at run-time.
-val create_in: i:index -> create_in_st i
 
 #restart-solver
 
