src/QUIC.Spec.fsti
@@ -1,7 +1,7 @@
 module QUIC.Spec
 
 include QUIC.Spec.Header.Base
-include QUIC.Crypto.Base
+include QUIC.Spec.Crypto
 
 module Seq = FStar.Seq
 module HD = Spec.Hash.Definitions
@@ -9,53 +9,6 @@ module AEAD = Spec.Agile.AEAD
 
 // JP: should we allow inversion on either hash algorithm or AEAD algorithm?
 #set-options "--max_fuel 0 --max_ifuel 0"
-
-// Move from Hashing.Spec to Spec.Hash?
-let keysized (a:ha) (l:nat) =
-  l <= HD.max_input_length a /\ l + HD.block_length a < pow2 32
-let hashable (a:ha) (l:nat) = l <= HD.max_input_length a
-
-let header_len_bound = 16500 // FIXME: this should be in line with the parser kind
-
-// AEAD plain and ciphertext. We want to guarantee that regardless
-// of the header size (max is 54), the neader + ciphertext + tag fits in a buffer
-// JP: perhaps cleaner with a separate lemma; any reason for putting this in a refinement?
-let max_plain_length: n:nat {
-  forall a. {:pattern AEAD.max_length a} n <= AEAD.max_length a
-} =
-  pow2 32 - header_len_bound - 16
-
-let max_cipher_length : n:nat {
-  forall a. {:pattern AEAD.max_length a \/ AEAD.tag_length a }
-    n <= AEAD.max_length a + AEAD.tag_length a
-} =
-  pow2 32 - header_len_bound
-
-type pbytes = b:bytes{let l = Seq.length b in 3 <= l /\ l < max_plain_length}
-type pbytes' (is_retry: bool) = b:bytes{let l = Seq.length b in if is_retry then l == 0 else (3 <= l /\ l < max_plain_length)}
-type cbytes = b:bytes{let l = Seq.length b in 19 <= l /\ l < max_cipher_length}
-type cbytes' (is_retry: bool) = b: bytes { let l = Seq.length b in if is_retry then l == 0 else (19 <= l /\ l < max_cipher_length) }
-
-// Static byte sequences to be fed into secret derivation. Marked as inline, so
-// that they can be used as arguments to gcmalloc_of_list for top-level arrays.
-inline_for_extraction
-val label_key: lbytes 3
-inline_for_extraction
-val label_iv: lbytes 2
-inline_for_extraction
-val label_hp: lbytes 2
-
-val derive_secret:
-  a: ha ->
-  prk:Spec.Hash.Definitions.bytes_hash a ->
-  label: bytes ->
-  len: nat ->
-  Ghost (* Pure *) (lbytes len)
-  (requires len <= 255 /\
-    Seq.length label <= 244 /\
-    keysized a (Seq.length prk)
-    )
-  (ensures fun out -> True)
 
 type nat2 = n:nat{n < 4}
 type nat4 = n:nat{n < 16}
