src/QUIC.Spec.Crypto.fst
@@ -1,0 +1,65 @@
+module QUIC.Spec.Crypto
+
+module U8 = FStar.UInt8
+module Seq = QUIC.Secret.Seq
+module HKDF = Spec.Agile.HKDF
+
+inline_for_extraction
+let prefix_l: List.Tot.llist U8.t 11 =
+  // JP: "tls13 quic "
+  [@inline_let]
+  let l = [0x74uy; 0x6cuy; 0x73uy; 0x31uy; 0x33uy;
+           0x20uy; 0x71uy; 0x75uy; 0x69uy; 0x63uy; 0x20uy] in
+  assert_norm (List.Tot.length l == 11);
+  l
+
+let prefix: lbytes 11 =
+  Seq.seq_of_list prefix_l
+
+#push-options "--z3rlimit 10"
+let lemma_hash_lengths (a:ha)
+  : Lemma (HD.hash_length a <= 64 /\ HD.word_length a <= 8 /\
+    HD.block_length a <= 128 /\ HD.max_input_length a >= pow2 61 - 1)
+  =
+  assert_norm(pow2 61 < pow2 125)
+#pop-options
+
+inline_for_extraction
+let label_key_l: List.Tot.llist U8.t 3 =
+  [@inline_let]
+  let l = [ 0x6buy; 0x65uy; 0x79uy ] in
+  assert_norm (List.Tot.length l = 3);
+  l
+
+let label_key =
+  Seq.seq_of_list label_key_l
+
+inline_for_extraction
+let label_iv_l: List.Tot.llist U8.t 2 =
+  [@inline_let]
+  let l = [ 0x69uy; 0x76uy ] in
+  assert_norm (List.Tot.length l = 2);
+  l
+
+let label_iv =
+  Seq.seq_of_list label_iv_l
+
+inline_for_extraction
+let label_hp_l: List.Tot.llist U8.t 2 =
+  [@inline_let]
+  let l = [ 0x68uy; 0x70uy ] in
+  assert_norm (List.Tot.length l = 2);
+  l
+
+let label_hp =
+  Seq.seq_of_list label_hp_l
+
+let derive_secret a prk label len =
+  let open Seq in
+  let z = Seq.create 1 0uy in
+  let lb = Seq.create 1 (U8.uint_to_t len) in // len <= 255
+  let llen = Seq.create 1 (U8.uint_to_t (11 + Seq.length label)) in
+  let info = z @| lb @| llen @| prefix @| label @| z in
+  lemma_hash_lengths a;
+  assert_norm(452 < pow2 61);
+  Seq.seq_reveal (HKDF.expand a prk (Seq.seq_hide info) len)
