src/QUIC.Spec.Crypto.fsti
@@ -1,0 +1,69 @@
+module QUIC.Spec.Crypto
+include QUIC.Spec.Base
+
+module Seq = FStar.Seq
+module HD = Spec.Hash.Definitions
+module AEAD = Spec.Agile.AEAD
+
+let supported_hash = function
+  | HD.SHA1 | HD.SHA2_256 | HD.SHA2_384 | HD.SHA2_512 -> true
+  | _ -> false
+
+let supported_aead = function
+  | AEAD.AES128_GCM | AEAD.AES256_GCM | AEAD.CHACHA20_POLY1305 -> true
+  | _ -> false
+
+type ha = a:HD.hash_alg{supported_hash a}
+type ea = a:AEAD.alg{supported_aead a}
+
+// JP: this is Spec.Agile.Cipher.key_length
+let ae_keysize (a:ea) =
+  match a with
+  | AEAD.AES128_GCM -> 16
+  | _ -> 32
+
+// Move from Hashing.Spec to Spec.Hash?
+let keysized (a:ha) (l:nat) =
+  l <= HD.max_input_length a /\ l + HD.block_length a < pow2 32
+let hashable (a:ha) (l:nat) = l <= HD.max_input_length a
+
+// AEAD plain and ciphertext. We want to guarantee that regardless
+// of the header size (max is 54), the neader + ciphertext + tag fits in a buffer
+// JP: perhaps cleaner with a separate lemma; any reason for putting this in a refinement?
+let max_plain_length: n:nat {
+  forall a. {:pattern AEAD.max_length a} n <= AEAD.max_length a
+} =
+  pow2 32 - header_len_bound - 16
+
+let max_cipher_length : n:nat {
+  forall a. {:pattern AEAD.max_length a \/ AEAD.tag_length a }
+    n <= AEAD.max_length a + AEAD.tag_length a
+} =
+  pow2 32 - header_len_bound
+
+type packet = b:bytes{let l = Seq.length b in (* 21 <= l /\ *) l < pow2 32}
+type pbytes = b:bytes{let l = Seq.length b in 3 <= l /\ l < max_plain_length}
+type pbytes' (is_retry: bool) = b:bytes{let l = Seq.length b in if is_retry then l == 0 else (3 <= l /\ l < max_plain_length)}
+type cbytes = b:bytes{let l = Seq.length b in 19 <= l /\ l < max_cipher_length}
+type cbytes' (is_retry: bool) = b: bytes { let l = Seq.length b in if is_retry then l == 0 else (19 <= l /\ l < max_cipher_length) }
+
+// Static byte sequences to be fed into secret derivation. Marked as inline, so
+// that they can be used as arguments to gcmalloc_of_list for top-level arrays.
+inline_for_extraction
+val label_key: lbytes 3
+inline_for_extraction
+val label_iv: lbytes 2
+inline_for_extraction
+val label_hp: lbytes 2
+
+val derive_secret:
+  a: ha ->
+  prk:Spec.Hash.Definitions.bytes_hash a ->
+  label: bytes ->
+  len: nat ->
+  Ghost (* Pure *) (lbytes len)
+  (requires len <= 255 /\
+    Seq.length label <= 244 /\
+    keysized a (Seq.length prk)
+    )
+  (ensures fun out -> True)
