Makefile
@@ -64,7 +64,7 @@ dist/Makefile.basic: $(filter-out %/prims.krml,$(ALL_KRML_FILES))
 	  -bundle LowStar.* \
 	  -bundle Prims,C.Failure,C,C.String,C.Loops,Spec.Loops,C.Endianness,FStar.*[rename=EverQuic_Kremlib] \
 	  -bundle 'Meta.*,Hacl.*,Vale.*,Spec.*,Lib.*,EverCrypt,EverCrypt.*[rename=EverQuic_EverCrypt]' \
-	  -bundle 'QUIC.Impl=QUIC.*[rename=EverQuic]'
+	  -bundle 'QUIC.Impl+QUIC.Impl.Crypto=QUIC.\*[rename=EverQuic,rename-prefix]'
 
 dist/libeverquic.a: dist/Makefile.basic
 	$(MAKE) -C dist -f Makefile.basic
